src/Examples/SouffleGeneratedCompiled/GraphCompiler.v
@@ -15,6 +15,6 @@ Definition topo_dims : GridGraph.Dimensions := [3; 3].
 
 (* No designated input/output nodes, so this uses [all_io_locations] -- every grid node is an
    input AND output for every relation. *)
-Definition compiled_graph := compile_program program_to_compile layout (all_io_locations program_to_compile layout topo_dims) (all_io_locations program_to_compile layout topo_dims) topo_dims (grid_fuel topo_dims).
+Definition compiled_graph := compile_program program_to_compile layout (all_io_locations program_to_compile layout topo_dims) (all_io_locations program_to_compile layout topo_dims) topo_dims.
 
 Eval vm_compute in compiled_graph.
